Apply code reviews

ArchSemArm/VMPromising.v
@@ -712,6 +712,12 @@ Definition prefix_to_va {n : N} (is_upper : bool) (p : bv n) : bv 64 :=
   let varange_bit := if is_upper then (bv_1 16) else (bv_0 16) in
   bv_concat 64 varange_bit (bv_concat 48 p (bv_0 (48 - n))).
 
+Definition is_upper_va (va : bv 64) : option bool :=
+  let top_bits := bv_extract 48 16 va in
+  if top_bits =? (-1)%bv then Some true
+  else if top_bits =? 0%bv then Some false
+  else None.
+
 Definition level_prefix {n : N} (va : bv n) (lvl : Level) : prefix lvl :=
   bv_extract (12 + 9 * (3 - lvl)) (9 * (lvl + 1)) va.
 
@@ -768,10 +774,12 @@ Module TLB.
   Module NDCtxt.
     Record t (lvl : Level) :=
       make {
+          is_upper : bool;
           va : prefix lvl;
           asid : option (bv 16);
         }.
     Arguments make {_} _ _.
+    Arguments is_upper {_}.
     Arguments va {_}.
     Arguments asid {_}.
 
@@ -783,8 +791,8 @@ Module TLB.
 
     #[global] Instance count lvl : Countable (t lvl).
     Proof.
-      eapply (inj_countable' (fun ndc => (va ndc, asid ndc))
-                        (fun x => make x.1 x.2)).
+      eapply (inj_countable' (fun ndc => (is_upper ndc, va ndc, asid ndc))
+                        (fun x => make x.1.1 x.1.2 x.2)).
       abstract sauto.
     Defined.
   End NDCtxt.
@@ -795,20 +803,17 @@ Module TLB.
     Definition nd (ctxt : t) : NDCtxt.t (lvl ctxt) := projT2 ctxt.
     Definition va (ctxt : t) : prefix (lvl ctxt) := NDCtxt.va (nd ctxt).
     Definition asid (ctxt : t) : option (bv 16) := NDCtxt.asid (nd ctxt).
+    Definition is_upper (ctxt : t) : bool := NDCtxt.is_upper (nd ctxt).
   End Ctxt.
   #[export] Typeclasses Transparent Ctxt.t.
 
   Module Entry.
-    Record t (lvl : Level) :=
+    Record t {lvl : Level} :=
       make {
-        is_upper : bool;
         val_ttbr : val;
         ptes : vec val (S lvl);
       }.
-    Arguments make {_} _ _ _.
-    Arguments is_upper {_}.
-    Arguments val_ttbr {_}.
-    Arguments ptes {_}.
+    Arguments t : clear implicits.
 
     #[global] Instance eq_dec lvl : EqDecision (t lvl).
     Proof. solve_decision. Defined.
@@ -818,18 +823,18 @@ Module TLB.
 
     #[global] Instance count lvl : Countable (t lvl).
     Proof.
-      eapply (inj_countable' (fun ent => (is_upper ent, val_ttbr ent, ptes ent))
-                        (fun x => make x.1.1 x.1.2 x.2)).
+      eapply (inj_countable' (fun ent => (val_ttbr ent, ptes ent))
+                        (fun x => make lvl x.1 x.2)).
       abstract sauto.
     Defined.
 
     Definition pte {lvl} (tlbe : t lvl) := Vector.last tlbe.(ptes).
 
     Program Definition append {lvl clvl : Level}
-        (tlbe : t lvl)
+        (tlbe : @t lvl)
         (pte : val)
-        (CHILD : lvl + 1 = clvl) : t clvl :=
-      make tlbe.(is_upper) tlbe.(val_ttbr) (ctrans _ (tlbe.(ptes) +++ [#pte])).
+        (CHILD : lvl + 1 = clvl) : @t clvl :=
+      make _ tlbe.(val_ttbr) (ctrans _ (tlbe.(ptes) +++ [#pte])).
     Solve All Obligations with lia.
   End Entry.
   Export (hints) Entry.
@@ -971,10 +976,10 @@ Module TLB.
       if (Memory.read_at loc init mem time) is Some (memval, _) then
         if decide (is_table memval) then
           let asid := bv_extract 48 16 val_ttbr in
-          let ndctxt := NDCtxt.make va (Some asid) in
+          let ndctxt := NDCtxt.make is_upper va (Some asid) in
           let ctxt := existT root_lvl ndctxt in
           let entry : Entry.t (Ctxt.lvl ctxt) :=
-            Entry.make is_upper val_ttbr ([#memval] : vec val (S root_lvl)) in
+            Entry.make _ val_ttbr ([#memval] : vec val (S root_lvl)) in
           (* add the entry to vatlb only when it is not in the original vatlb *)
           if decide (entry ∉ (VATLB.get ctxt vatlb)) then
             Ok (VATLB.insert ctxt entry vatlb, true)
@@ -998,11 +1003,6 @@ Module TLB.
       (te : Entry.t (Ctxt.lvl ctxt))
       (index : bv 9)
       (ttbr : reg) : result string (VATLB.t * bool) :=
-    (* guard_or "ASID is not active"
-      $ is_active_asid ts (Ctxt.asid ctxt) ttbr time;; *)
-    guard_or "The translation entry is not in the TLB"
-      (te ∈ VATLB.get ctxt vatlb);;
-
     if decide (¬is_table (Entry.pte te)) then Ok (vatlb, false)
     else
       let entry_addr := next_entry_addr (Entry.pte te) index in
@@ -1015,7 +1015,7 @@ Module TLB.
           let va := next_va ctxt index (child_lvl_add_one _ _ e) in
           let asid := if bool_decide (is_global clvl next_pte) then None
                       else Ctxt.asid ctxt in
-          let ndctxt := NDCtxt.make va asid in
+          let ndctxt := NDCtxt.make (Ctxt.is_upper ctxt) va asid in
           let ctxt := existT clvl ndctxt in
           let entry := Entry.append te next_pte (child_lvl_add_one _ _ e) in
           (* add the entry to vatlb only when it is not in the original vatlb *)
@@ -1047,11 +1047,12 @@ Module TLB.
         let index := level_index va lvl in
         sregs ← othrow "TTBR should exist in initial state"
                 $ TState.read_sreg_at ts ttbr time;
+        is_upper ← othrow "The register is not TTBR" (is_upper_ttbr ttbr);
         foldlM (λ prev sreg,
           val_ttbr ← othrow "TTBR should be a 64 bit value"
                   $ regval_to_val ttbr sreg.1;
           let asid := bv_extract 48 16 val_ttbr in
-          let ndctxt := NDCtxt.make pva (Some asid) in
+          let ndctxt := NDCtxt.make is_upper pva (Some asid) in
           let ctxt := existT plvl ndctxt in
           (* parent entries should be from the original TLB (in the parent level) *)
           let tes := elements (VATLB.get ctxt tlb.(vatlb)) in
@@ -1194,7 +1195,6 @@ Module TLB.
     | (ev, t) :: tl =>
       match ev with
       | Ev.Tlbi tlbi =>
-        let va := prefix_to_va (Entry.is_upper te) (Ctxt.va ctxt) in
         if decide (is_te_invalidated_by_tlbi tlbi tid ctxt te) then
           mret (Some t)
         else
@@ -1239,8 +1239,10 @@ Module TLB.
               (lvl : Level)
               (va : bv 64) (asid : bv 16) :
             result string (list (val * list val * (option nat))) :=
-    let ndctxt_asid := NDCtxt.make (level_prefix va lvl) (Some asid) in
-    let ndctxt_global := NDCtxt.make (level_prefix va lvl) None in
+    is_upper ← othrow ("VA is not in the range: " ++ (pretty va))%string
+                (is_upper_va va);
+    let ndctxt_asid := NDCtxt.make is_upper (level_prefix va lvl) (Some asid) in
+    let ndctxt_global := NDCtxt.make is_upper (level_prefix va lvl) None in
     candidates_asid ←
       get_leaf_ptes_with_inv_time_by_ctxt mem tid tlb trans_time lvl ndctxt_asid;
     candidates_global ←
@@ -1277,7 +1279,9 @@ Module TLB.
                 (ttbr : reg) :
         result string (list (val * list val * (option nat))) :=
     if parent_lvl lvl is Some parent_lvl then
-      let ndctxt := NDCtxt.make (level_prefix va parent_lvl) asid in
+      is_upper ← othrow ("VA is not in the range: " ++ (pretty va))%string
+                (is_upper_va va);
+      let ndctxt := NDCtxt.make is_upper (level_prefix va parent_lvl) asid in
       let ctxt := existT parent_lvl ndctxt in
       let tes := VATLB.get ctxt tlb.(TLB.vatlb) in
       let tes := filter (λ te, is_table (TLB.Entry.pte te)) tes in
@@ -1376,7 +1380,7 @@ Module TLB.
       candidates ← TLB.lookup mem tid tlb trans_time va asid;
       let new :=
         omap (λ '(val_ttbr, path, ti_opt),
-          if (is_new_entry val_ttbr path ti_opt entries) then
+          if is_new_entry val_ttbr path ti_opt entries then
             Some (val_ttbr, path, trans_time, ti_opt)
           else None
         ) candidates in
@@ -1397,7 +1401,7 @@ Module TLB.
         candidates ← TLB.get_invalid_ptes_with_inv_time ts init mem tid tlb trans_time va asid ttbr;
         let new :=
           omap (λ '(val_ttbr, path, ti_opt),
-            if decide (is_new_entry val_ttbr path ti_opt entries) then
+            if is_new_entry val_ttbr path ti_opt entries then
               Some (val_ttbr, path, trans_time, ti_opt)
             else None
           ) candidates in
@@ -1420,8 +1424,7 @@ Module IIS.
           va : bv 36;
           time : nat;
           root : option {ttbr : reg & reg_type ttbr};
-          remaining : list (bv 64);
-          invalidation : option nat
+          remaining : list (bv 64)
         }.
 
     Definition pop : Exec.t t string (bv 64) :=
@@ -1436,10 +1439,11 @@ Module IIS.
     make {
         strict : view;
         (* The translations results of the latest translation *)
-        trs : option TransRes.t
+        trs : option TransRes.t;
+        inv_time : option nat
       }.
 
-  Definition init : t := make 0 None.
+  Definition init : t := make 0 None None.
 
   (** Add a new view to the IIS *)
   Definition add (v : view) (iis : t) : t :=
@@ -1447,6 +1451,9 @@ Module IIS.
 
   Definition set_trs (tres : TransRes.t) :=
     setv trs (Some tres).
+
+  Definition set_inv_time (ti_opt : option nat) :=
+    setv inv_time ti_opt.
 
 End IIS.
 
@@ -1520,14 +1527,17 @@ Definition run_reg_general_read (reg : reg) (racc : reg_acc) :
 Definition run_reg_trans_read (reg : reg) (racc : reg_acc)
       (trs : IIS.TransRes.t) :
     Exec.t TState.t string (reg_type reg * view) :=
-  guard_or "Translation read during the translation should be implicit"
+  guard_or "Register read during the translation should be implicit"
     (¬ (is_Some racc));;
   root ← othrow "Could not find the translation root: error in translation assumptions"
     (trs.(IIS.TransRes.root));
-  if decide (projT1 root = reg) is left eq then
-    mret (ctrans eq (projT2 root), 0%nat)
+  if decide (root.T1 = reg) is left eq then
+    mret (ctrans eq root.T2, 0%nat)
   else
     ts ← mGet;
+    guard_or
+      ("The register should niether be relaxed nor strict: " ++ pretty reg)%string
+      $ (reg ∉ strict_regs ∨ reg ∉ relaxed_regs);;
     othrow
       ("Register " ++ pretty reg ++ " unmapped; cannot read")%string
       $ TState.read_reg ts reg.
@@ -1588,18 +1598,14 @@ Definition run_mem_read (addr : address) (macc : mem_acc) (init : Memory.initial
   iis ← mget PPState.iis;
   let vaddr := iis.(IIS.strict) in
   if is_explicit macc then
-    tres_opt ← mget (IIS.trs ∘ PPState.iis);
-    trans_res ← othrow "Explicit access before translation" tres_opt;
-    let invalidation := trans_res.(IIS.TransRes.invalidation) in
     '(view, val) ←
       Exec.liftSt (PPState.state ×× PPState.mem)
-        $ read_mem_explicit loc vaddr invalidation macc init;
+        $ read_mem_explicit loc vaddr iis.(IIS.inv_time) macc init;
     mset PPState.iis $ IIS.add view;;
     mret val
   else if is_ttw macc then
     ts ← mget PPState.state;
-    tres_option ← mget (IIS.trs ∘ PPState.iis);
-    tres ← othrow "TTW read before translation start" tres_option;
+    tres ← othrow "TTW read before translation start" iis.(IIS.trs);
     '(view, val) ←
       read_pte vaddr (ts, tres)
       |> Exec.lift_res_set_full
@@ -1828,27 +1834,28 @@ Definition run_trans_start (trans_start : TranslationStartInfo)
       valid_entries ← mlift $ TLB.get_valid_entries_from_snapshots snapshots mem tid va asid;
       invalid_entries ← mlift $
         TLB.get_invalid_entries_from_snapshots snapshots ts init mem tid is_ets2 va asid ttbr;
-      (* update IIS with either a valid translation result or a fault *)
-      valid_trs ←
+      (* update IIS with either a valid translation result or an invalid result *)
+      valid_res ←
         for (val_ttbr, path, t, ti) in valid_entries do
           val_ttbr ← othrow
             "TTBR value type does not match with the value from the translation"
             (val_to_regval ttbr val_ttbr);
           let root := (Some (existT ttbr val_ttbr)) in
-          mret $ IIS.TransRes.make (va_to_vpn va) t root path ti
+          mret $ (IIS.TransRes.make (va_to_vpn va) t root path, ti)
         end;
-      invalid_trs ←
+      invalid_res ←
         for (val_ttbr, path, t, ti) in invalid_entries do
           val_ttbr ← othrow
             "TTBR value type does not match with the value from the translation"
             (val_to_regval ttbr val_ttbr);
           let root := (Some (existT ttbr val_ttbr)) in
-          mret $ IIS.TransRes.make (va_to_vpn va) t root path ti
+          mret $ (IIS.TransRes.make (va_to_vpn va) t root path, ti)
         end;
-      mchoosel (valid_trs ++ invalid_trs)
+      mchoosel (valid_res ++ invalid_res)
     else
-      mret $ IIS.TransRes.make (va_to_vpn va) vpre_t None [] None;
-  mset PPState.iis $ IIS.set_trs trans_res.
+      mret $ (IIS.TransRes.make (va_to_vpn va) vpre_t None [], None);
+  mset PPState.iis $ IIS.set_trs trans_res.1;;
+  mset PPState.iis $ IIS.set_inv_time trans_res.2.
 
 Definition read_fault_vpre (is_acq : bool)
   (trans_time : nat) : Exec.t (TState.t * IIS.t) string view :=
@@ -1876,7 +1883,7 @@ Definition run_trans_end (trans_end : trans_end) :
     let trans_time := trs.(IIS.TransRes.time) in
     let fault := trans_end.(AddressDescriptor_fault) in
     if decide (fault.(FaultRecord_statuscode) = Fault_None) then
-      mret ()
+      mset snd $ setv IIS.trs None
     else
       is_ets3 ← mlift (ets3 ts);
       if is_ets3 && (trans_time <? (ts.(TState.vrd) ⊔ ts.(TState.vwr)))
@@ -1893,16 +1900,18 @@ Definition run_trans_end (trans_end : trans_end) :
         let is_write := fault.(FaultRecord_access).(AccessDescriptor_write) in
         let is_rel := fault.(FaultRecord_access).(AccessDescriptor_relsc) in
         write_view ← write_fault_vpre is_rel trans_time;
-        mset snd $ IIS.add (view_if is_write write_view)
+        mset snd $ IIS.add (view_if is_write write_view);;
+        mset snd $ setv IIS.trs None
   else
     mthrow "Translation ends with an empty translation".
 
+(* TODO: check translation fault using `fault` and handle other cases *)
 Definition run_take_exception (fault : exn) (vmax_t : view) :
     Exec.t (TState.t * IIS.t) string () :=
   iis ← mget snd;
   if iis.(IIS.trs) is Some trans_res then
-    match trans_res.(IIS.TransRes.invalidation) with
-    | Some invalidation => run_cse invalidation
+    match iis.(IIS.inv_time) with
+    | Some inv_time => run_cse inv_time
     | None => mret ()
     end
   else
@@ -1940,11 +1949,9 @@ Section RunOutcome.
       addr ← othrow "Address not supported" $ Loc.from_addr addr;
       viio ← mget (IIS.strict ∘ PPState.iis);
       if is_explicit macc then
-        tres_opt ← mget (IIS.trs ∘ PPState.iis);
-        trans_res ← othrow "Explicit access before translation" tres_opt;
-        let invalidation := trans_res.(IIS.TransRes.invalidation) in
+        inv_time ← mget (IIS.inv_time ∘ PPState.iis);
         vpre_opt ← Exec.liftSt (PPState.state ×× PPState.mem) $
-                      write_mem_xcl tid addr viio invalidation macc val;
+                      write_mem_xcl tid addr viio inv_time macc val;
         mret (Ok (), vpre_opt)
       else mthrow "Unsupported non-explicit write"
   | MemWrite _ _ _ => mthrow "Memory write of size other than 8, or with tags"
